Evaluation Value Remains Same
Added a new lemma 'stay_same' (name WIP) that states that
if no nodes that a nid uses (including the nid itself) changes
(where changes means that the IRNode type is different) between
graphs, then the evaluated value will be the same in both graphs.

Used this lemma to finish the eval_independent lemma.

Currently stuck on trying to prove nodes which use 'nid' in their
premises, for some reason the induction tactic refuses to consider
the nid identifier in the premises as equal to nid in the conclusion.
Configuring IRNode's to hold the nid does resolve this issue but
needlessly duplicates the state.

Canonicalization.thy
@@ -198,6 +198,35 @@ inductive eval_uses:: "IRGraph \<Rightarrow> ID \<Rightarrow> ID \<Rightarrow> b
     eval_uses g nid' nid''\<rbrakk>
     \<Longrightarrow> eval_uses g nid nid''"
 
+fun eval_usages :: "IRGraph \<Rightarrow> ID \<Rightarrow> ID set" where
+  "eval_usages g nid = set (filter (eval_uses g nid) (sorted_list_of_set (ids g)))"
+
+lemma eval_usages[simp]:
+  assumes "us = eval_usages g nid"
+  assumes "nid' \<in> ids g"
+  shows "eval_uses g nid nid' \<longleftrightarrow> nid' \<in> us" (is "?P \<longleftrightarrow> ?Q")
+  using assms eval_usages.simps by simp
+
+lemma inputs_are_uses:
+  assumes "nid' \<in> set (inputs_of (kind g nid))"
+  shows "eval_uses g nid nid'"
+  using assms eval_uses.intros(1) by blast
+
+lemma inputs_are_usages:
+  assumes "nid' \<in> set (inputs_of (kind g nid))"
+  assumes "nid' \<in> ids g"
+  shows "nid' \<in> eval_usages g nid"
+  using assms(1) assms(2) eval_usages inputs_are_uses by blast
+
+lemma usage_includes_inputs:
+  assumes "us = eval_usages g nid"
+  assumes "ls = set (inputs_of (kind g nid))"
+  assumes "ls \<subseteq> ids g"
+  shows "ls \<subseteq> us"
+  using inputs_are_usages eval_usages
+  using assms(1) assms(2) assms(3) by blast
+
+
 lemma kind_uneffected:
   assumes oldnid: "nid \<in> ids g"
   assumes newnid: "newnid \<notin> ids g"
@@ -207,6 +236,17 @@ proof -
   have uneq: "nid \<noteq> newnid"
     using newnid oldnid by blast
   show ?thesis using uneq modg
+    apply (simp add: Abs_IRGraph_inverse snd.rep_eq)
+    using irgraph_dom
+    by (smt finsert_iff fun_upd_same fun_upd_triv fun_upd_twist ids.simps irgraph_dom_inv irgraph_dom_x irgraph_rng notin_fset option.discI snd.rep_eq)
+qed
+
+lemma kind_uneffected_uneq:
+  assumes "nid \<noteq> newnid"
+  assumes modg: "modg = add_node newnid anyk g"
+  shows "(kind g nid) = (kind modg nid)"
+proof -
+  show ?thesis using assms modg
     apply (simp add: Abs_IRGraph_inverse snd.rep_eq)
     using irgraph_dom
     by (smt finsert_iff fun_upd_same fun_upd_triv fun_upd_twist ids.simps irgraph_dom_inv irgraph_dom_x irgraph_rng notin_fset option.discI snd.rep_eq)
@@ -233,9 +273,251 @@ proof -
     by (smt finsert_iff fun_upd_apply ids.simps irgraph_dom_inv irgraph_dom_x irgraph_rng notin_fset option.case_eq_if option.discI option.sel)
 qed
 
+fun changes :: "ID \<Rightarrow> IRGraph \<Rightarrow> IRGraph \<Rightarrow> bool" where
+  "changes nid g1 g2 = ((kind g1 nid) \<noteq> (kind g2 nid))"
+
+lemma add_node_changes:
+  assumes "nid \<notin> ids g1"
+  assumes "n \<noteq> NoNode"
+  assumes "g2 = add_node nid n g1"
+  shows "changes nid g1 g2"
+  using add_implies_kind assms(1) assms(2) assms(3) irgraph_dom_inv by auto
+
+lemma remove_node_effect:
+  assumes "g2 = remove_node nid g1"
+  shows "kind g2 nid = NoNode"
+  using Rep_IRGraph assms fst.rep_eq snd.rep_eq by auto
+
+lemma remove_node_changes:
+  assumes "nid \<in> ids g1"
+  assumes "kind g1 nid \<noteq> NoNode"
+  assumes "g2 = remove_node nid g1"
+  shows "changes nid g1 g2"
+  using assms(2) assms(3) remove_node_effect by auto
+
+lemma kind_floats:
+  assumes "g1 m \<turnstile> nid (kind g1 nid) \<mapsto> v1"
+  shows "is_floating_node (kind g1 nid)"
+  using assms evalFloating by blast
+
+lemma unchanged_implies_unchanged_inputs:
+  assumes "\<forall> nid' \<in> (eval_usages g1 nid) . \<not>(changes nid' g1 g2)"
+  shows "\<forall> nid' \<in> (eval_usages g1 nid) . (\<forall> nid'' \<in> (eval_usages g1 nid') . \<not>(changes nid'' g1 g2))"
+  by (metis assms eval_usages.simps eval_uses.intros(2) filter_set member_filter)
+
+lemma stay_same:
+  assumes "\<not>(changes nid g1 g2)"
+  assumes "\<forall> nid' \<in> (eval_usages g1 nid) . \<not>(changes nid' g1 g2)"
+  assumes "g1 m \<turnstile> nid (kind g1 nid) \<mapsto> v1"
+  shows "g2 m \<turnstile> nid (kind g2 nid) \<mapsto> v1" 
+proof -
+  have kind_same: "kind g1 nid = kind g2 nid"
+    using assms(1) by auto
+
+  show ?thesis using assms(3) assms(1) assms(2) kind_same
+proof (induct m nid "kind g1 nid" v1 arbitrary: nid rule: "eval.induct")
+  case const: (ConstantNode val c)
+  then have "kind g2 nid = (ConstantNode c)"
+    using kind_same by presburger
+  then show ?case
+    by (simp add: const.hyps(1) eval.ConstantNode)
+next
+  case param: (ParameterNode val m i nid)
+  show ?case
+    using eval.ParameterNode param.hyps(1) param.hyps(2) param.prems(3) by fastforce
+next
+  case phi: (PhiNode val m nid uu)
+  then have kind: "kind g2 nid = (PhiNode uu)"
+    by presburger
+  then have "g1 m \<turnstile> nid (kind g1 nid) \<mapsto> val"
+    using PhiNode phi.hyps(1) sorry
+  then show ?case
+    using PhiNode kind phi.prems(3) by auto
+next
+  case (ValuePhiNode val m nid uv uw)
+  then have kind: "kind g2 nid = (ValuePhiNode uv uw)"
+    by presburger
+  then have "g1 m \<turnstile> nid (kind g1 nid) \<mapsto> val"
+    sorry
+  then show ?case
+    using ValuePhiNode.prems(3) kind eval.ValuePhiNode by auto
+next
+  case (ValueProxyNode m c val nid u)
+  then have "g2 m \<turnstile> c (kind g2 c) \<mapsto> val"
+    by (smt changes.simps eval_usages.simps eval_uses.intros(2) filter_set inputs_are_usages inputs_of.simps(12) list.set_intros(1) member_filter not_in_no_val set_subset_Cons subsetD)
+  then show ?case
+    by (metis ValueProxyNode.hyps(3) ValueProxyNode.prems(3) eval.ValueProxyNode)
+next
+  case (AbsNode m x v nid)
+  then have "g2 m \<turnstile> x (kind g2 x) \<mapsto> IntVal v"
+    by (metis changes.simps eval_usages.simps eval_uses.intros(2) filter_set inputs_are_usages inputs_of.simps(3) list.set_intros(1) member_filter not_in_no_val)
+  then show ?case
+    using AbsNode.hyps(3) AbsNode.prems(3) eval.AbsNode by fastforce
+next
+  case (NegateNode m x v nid)
+  then have "g1 m \<turnstile> x (kind g1 x) \<mapsto> IntVal v"
+    by presburger
+  then have "g2 m \<turnstile> x (kind g2 x) \<mapsto> IntVal v"
+    using unchanged_implies_unchanged_inputs assms
+    by (metis NegateNode.hyps(2) NegateNode.hyps(3) NegateNode.prems(2) changes.elims(3) inputs_are_usages inputs_of.simps(26) list.set_intros(1) not_in_no_val)
+  then show ?case
+    using NegateNode.hyps(3) NegateNode.prems(3) eval.NegateNode by fastforce
+next
+  case (AddNode m x v1 y v2 nid)
+  then have "g1 m \<turnstile> x (kind g1 x) \<mapsto> IntVal v1"
+    by blast
+  then have v1: "g2 m \<turnstile> x (kind g2 x) \<mapsto> IntVal v1"
+    using unchanged_implies_unchanged_inputs
+    by (metis AddNode.hyps(2) AddNode.hyps(5) AddNode.prems(2) changes.elims(3) inputs_are_usages inputs_of.simps(23) list.set_intros(1) not_in_no_val)
+  have "g1 m \<turnstile> y (kind g1 y) \<mapsto> IntVal v2"
+    using AddNode.hyps(3) by simp
+  then have v2: "g2 m \<turnstile> y (kind g2 y) \<mapsto> IntVal v2"
+    using unchanged_implies_unchanged_inputs
+    by (metis AddNode.hyps(4) AddNode.hyps(5) AddNode.prems(2) changes.simps in_set_member inputs_are_usages inputs_of.simps(23) member_rec(1) not_in_no_val)
+  then show ?case using v1 v2
+    using AddNode.hyps(5) AddNode.prems(3) eval.AddNode by fastforce
+next
+  case (SubNode m x v1 y v2 nid)
+  then have "g1 m \<turnstile> x (kind g1 x) \<mapsto> IntVal v1"
+    by blast
+  then have v1: "g2 m \<turnstile> x (kind g2 x) \<mapsto> IntVal v1"
+    by (metis SubNode.hyps(2) SubNode.hyps(5) SubNode.prems(2) changes.elims(3) inputs_are_usages inputs_of.simps(1) list.set_intros(1) not_in_no_val unchanged_implies_unchanged_inputs)
+  have "g1 m \<turnstile> y (kind g1 y) \<mapsto> IntVal v2"
+    using SubNode.hyps(3) by auto
+  then have v2: "g2 m \<turnstile> y (kind g2 y) \<mapsto> IntVal v2"
+    by (metis SubNode.hyps(4) SubNode.hyps(5) SubNode.prems(2) changes.simps in_set_member inputs_are_usages inputs_of.simps(1) member_rec(1) not_in_no_val unchanged_implies_unchanged_inputs)
+  then show ?case using v1 v2
+    using SubNode.hyps(5) SubNode.prems(3) eval.SubNode by fastforce
+next
+  case node: (MulNode m x v1 y v2 nid)
+  then have "g1 m \<turnstile> x (kind g1 x) \<mapsto> IntVal v1"
+    by blast
+  then have v1: "g2 m \<turnstile> x (kind g2 x) \<mapsto> IntVal v1"
+    by (metis node.hyps(2) node.hyps(5) node.prems(2) changes.elims(3) inputs_are_usages inputs_of.simps(37) list.set_intros(1) not_in_no_val unchanged_implies_unchanged_inputs)
+  have "g1 m \<turnstile> y (kind g1 y) \<mapsto> IntVal v2"
+    using node.hyps(3) by auto
+  then have v2: "g2 m \<turnstile> y (kind g2 y) \<mapsto> IntVal v2"
+    by (metis (no_types, lifting) node.hyps(4) node.hyps(5) node.prems(2) changes.simps eval_usages.simps eval_uses.intros(2) filter_set in_set_member inputs_are_usages inputs_of.simps(37) member_filter member_rec(1) not_in_no_val)
+  then show ?case using v1 v2
+    using node.hyps(5) node.prems(3) eval.MulNode by fastforce
+next
+  case node: (AndNode m x v1 y v2 nid)
+  then have "g1 m \<turnstile> x (kind g1 x) \<mapsto> IntVal v1"
+    by blast
+  then have v1: "g2 m \<turnstile> x (kind g2 x) \<mapsto> IntVal v1"
+    by (metis changes.elims(3) inputs_are_usages inputs_of.simps(35) list.set_intros(1) node.hyps(2) node.hyps(5) node.prems(2) not_in_no_val unchanged_implies_unchanged_inputs)
+  have "g1 m \<turnstile> y (kind g1 y) \<mapsto> IntVal v2"
+    using node.hyps(3) by auto
+  then have v2: "g2 m \<turnstile> y (kind g2 y) \<mapsto> IntVal v2"
+    by (metis (no_types, lifting) changes.simps eval_usages.simps eval_uses.intros(2) filter_set in_set_member inputs_are_usages inputs_of.simps(35) member_filter member_rec(1) node.hyps(4) node.hyps(5) node.prems(2) not_in_no_val)
+  then show ?case using v1 v2
+    using node.hyps(5) node.prems(3) eval.AndNode by fastforce
+next
+  case node: (OrNode m x v1 y v2 nid)
+  then have "g1 m \<turnstile> x (kind g1 x) \<mapsto> IntVal v1"
+    by blast
+  then have v1: "g2 m \<turnstile> x (kind g2 x) \<mapsto> IntVal v1"
+    by (metis changes.elims(3) inputs_are_usages inputs_of.simps(10) list.set_intros(1) node.hyps(2) node.hyps(5) node.prems(2) not_in_no_val unchanged_implies_unchanged_inputs)
+  have "g1 m \<turnstile> y (kind g1 y) \<mapsto> IntVal v2"
+    using node.hyps(3) by auto
+  then have v2: "g2 m \<turnstile> y (kind g2 y) \<mapsto> IntVal v2"
+    by (metis (no_types, lifting) changes.simps eval_usages.simps eval_uses.intros(2) filter_set in_set_member inputs_are_usages inputs_of.simps(10) member_filter member_rec(1) node.hyps(4) node.hyps(5) node.prems(2) not_in_no_val)
+  then show ?case using v1 v2
+    using node.hyps(5) node.prems(3) eval.OrNode by fastforce
+next
+  case node: (XorNode m x v1 y v2 nid)
+  then have "g1 m \<turnstile> x (kind g1 x) \<mapsto> IntVal v1"
+    by blast
+  then have v1: "g2 m \<turnstile> x (kind g2 x) \<mapsto> IntVal v1"
+    by (metis changes.elims(3) inputs_are_usages inputs_of.simps(22) list.set_intros(1) node.hyps(2) node.hyps(5) node.prems(2) not_in_no_val unchanged_implies_unchanged_inputs)  
+  have "g1 m \<turnstile> y (kind g1 y) \<mapsto> IntVal v2"
+    using node.hyps(3) by auto
+  then have v2: "g2 m \<turnstile> y (kind g2 y) \<mapsto> IntVal v2"
+    by (metis (no_types, lifting) changes.simps eval_usages.simps eval_uses.intros(2) filter_set in_set_member inputs_are_usages inputs_of.simps(22) member_filter member_rec(1) node.hyps(4) node.hyps(5) node.prems(2) not_in_no_val)
+  then show ?case using v1 v2
+    using node.hyps(5) node.prems(3) eval.XorNode by fastforce
+next
+  case node: (IntegerEqualsNode m x v1 y v2 val nid)
+  then have "g1 m \<turnstile> x (kind g1 x) \<mapsto> IntVal v1"
+    by blast
+  then have v1: "g2 m \<turnstile> x (kind g2 x) \<mapsto> IntVal v1"
+    by (metis changes.elims(3) inputs_are_usages inputs_of.simps(40) list.set_intros(1) node.hyps(2) node.hyps(6) node.prems(2) not_in_no_val unchanged_implies_unchanged_inputs)
+  have "g1 m \<turnstile> y (kind g1 y) \<mapsto> IntVal v2"
+    using node.hyps(3) by auto
+  then have v2: "g2 m \<turnstile> y (kind g2 y) \<mapsto> IntVal v2"
+    by (metis (no_types, lifting) changes.simps eval_usages.simps eval_uses.intros(2) filter_set in_set_member inputs_are_usages inputs_of.simps(40) member_filter member_rec(1) node.hyps(4) node.hyps(6) node.prems(2) not_in_no_val)
+  then show ?case using v1 v2
+    using IntegerEqualsNode node.hyps(5) node.hyps(6) node.prems(3) by fastforce
+next
+  case node: (IntegerLessThanNode m x v1 y v2 val nid)
+  then have "g1 m \<turnstile> x (kind g1 x) \<mapsto> IntVal v1"
+    by blast
+  then have v1: "g2 m \<turnstile> x (kind g2 x) \<mapsto> IntVal v1"
+    by (metis (no_types, lifting) changes.simps eval_usages.simps eval_uses.intros(2) filter_set inputs_are_usages inputs_of.simps(51) list.set_intros(1) member_filter node.hyps(2) node.hyps(6) node.prems(2) not_in_no_val)
+  have "g1 m \<turnstile> y (kind g1 y) \<mapsto> IntVal v2"
+    using node.hyps(3) by auto
+  then have v2: "g2 m \<turnstile> y (kind g2 y) \<mapsto> IntVal v2"
+    by (metis (no_types, lifting) changes.simps eval_usages.simps eval_uses.intros(2) filter_set in_set_member inputs_are_usages inputs_of.simps(51) member_filter member_rec(1) node.hyps(4) node.hyps(6) node.prems(2) not_in_no_val)
+  then show ?case using v1 v2
+    using IntegerLessThanNode node.hyps(5) node.hyps(6) node.prems(3) by fastforce
+next
+  case (ConditionalNode m condition cond trueExp trueVal falseExp falseVal val nid)
+  have trueVal: "g2 m \<turnstile> trueExp (kind g2 trueExp) \<mapsto> IntVal(trueVal)"
+    by (metis (no_types, lifting) ConditionalNode.hyps(3) ConditionalNode.hyps(4) ConditionalNode.hyps(8) ConditionalNode.prems(2) changes.simps eval_usages.simps eval_uses.intros(2) filter_set in_set_member inputs_are_usages inputs_of.simps(29) member_filter member_rec(1) not_in_no_val)
+  have falseVal: "g2 m \<turnstile> falseExp (kind g2 falseExp) \<mapsto> IntVal(falseVal)"
+    by (metis (no_types, lifting) ConditionalNode.hyps(5) ConditionalNode.hyps(6) ConditionalNode.hyps(8) ConditionalNode.prems(2) changes.simps eval_usages.simps eval_uses.intros(2) filter_set in_set_member inputs_are_usages inputs_of.simps(29) member_filter member_rec(1) not_in_no_val)
+  have cond: "g2 m \<turnstile> condition (kind g2 condition) \<mapsto> IntVal(cond)"
+    by (metis ConditionalNode.hyps(1) ConditionalNode.hyps(2) ConditionalNode.hyps(8) ConditionalNode.prems(2) changes.simps inputs_are_usages inputs_of.simps(29) list.set_intros(1) not_in_no_val unchanged_implies_unchanged_inputs)
+  have "g2 m \<turnstile> nid (kind g2 nid) \<mapsto> val"
+    using kind_same trueVal falseVal cond
+    using ConditionalNode.hyps(7) ConditionalNode.hyps(8) ConditionalNode.prems(1) eval.ConditionalNode by fastforce
+  then show ?case
+    by blast
+next
+  case node: (ShortCircuitOrNode m x v1 y v2 val nid)
+  then have "g1 m \<turnstile> x (kind g1 x) \<mapsto> IntVal v1"
+    by blast
+  then have v1: "g2 m \<turnstile> x (kind g2 x) \<mapsto> IntVal v1"
+    by (metis changes.elims(3) inputs_are_usages inputs_of.simps(13) list.set_intros(1) node.hyps(2) node.hyps(6) node.prems(2) not_in_no_val unchanged_implies_unchanged_inputs)
+  have "g1 m \<turnstile> y (kind g1 y) \<mapsto> IntVal v2"
+    using node.hyps(3) by auto
+  then have v2: "g2 m \<turnstile> y (kind g2 y) \<mapsto> IntVal v2"
+    by (metis (no_types, lifting) changes.simps eval_usages.simps eval_uses.intros(2) filter_set in_set_member inputs_are_usages inputs_of.simps(13) member_filter member_rec(1) node.hyps(4) node.hyps(6) node.prems(2) not_in_no_val)
+  then show ?case using v1 v2
+    using eval.ShortCircuitOrNode node.hyps(5) node.hyps(6) node.prems(3) by fastforce
+next
+  case node: (LogicNegationNode m x v1 val nid)
+  then have "g1 m \<turnstile> x (kind g1 x) \<mapsto> IntVal v1"
+    by blast
+  then have v1: "g2 m \<turnstile> x (kind g2 x) \<mapsto> IntVal v1"
+    by (metis changes.elims(3) inputs_are_usages inputs_of.simps(50) list.set_intros(1) node.hyps(2) node.hyps(4) node.prems(2) not_in_no_val unchanged_implies_unchanged_inputs)
+  then show ?case using v1
+    using LogicNegationNode node.hyps(3) node.hyps(4) node.prems(3) by fastforce
+next
+  case (CallNodeEval val m nid start args children)
+  then show ?case sorry
+next
+  case (RefNode m x val nid)
+  then show ?case
+    by (metis changes.simps eval.RefNode eval_usages.simps eval_uses.intros(2) filter_set inputs_are_usages inputs_of.simps(56) list.set_intros(1) member_filter not_in_no_val)
+qed
+qed
+
+lemma eval_uses_to_changes:
+  assumes "nid \<noteq> nid'"
+  assumes "\<not>(eval_uses g1 nid nid')"
+  assumes "g2 = add_node nid' n g1"
+  shows "\<not>(changes nid g1 g2) \<and> (\<forall> nid' \<in> (eval_usages g1 nid) . \<not>(changes nid' g1 g2))" (is "?P \<and> ?Q")
+proof
+  show ?P
+    using assms(1) assms(3) changes.simps kind_uneffected_uneq by blast
+next
+  show ?Q 
+    by (metis assms(2) assms(3) changes.elims(2) eval_usages.simps filter_set kind_uneffected_uneq member_filter)
+qed
+
 lemma eval_independent:
   assumes indep: "\<not>(eval_uses g1 nid nid') \<and> nid \<noteq> nid'"
-  assumes not_in: "nid' \<notin> ids g1"
   assumes g2: "g2 = add_node nid' n g1"
   assumes v1: "g1 m \<turnstile> nid (kind g1 nid) \<mapsto> v1"
   shows "g2 m \<turnstile> nid (kind g2 nid) \<mapsto> v1"
@@ -243,13 +525,13 @@ proof -
   have nid_in: "nid \<in> ids g1"
     using not_in_no_val v1 by blast
   then have k: "(kind g1 nid) = (kind g2 nid)"
-    using kind_uneffected not_in
-    using g2 by blast
+    using g2 indep kind_uneffected_uneq by blast
   show ?thesis
   proof (cases "is_floating_node (kind g2 nid)")
     case True
     then show ?thesis
-      apply (cases "kind g2 nid"; auto) sorry
+      using eval_uses_to_changes indep g2 v1 stay_same
+      by meson
   next
     case False
     then show ?thesis
